{-# OPTIONS --without-K --rewriting #-}
module ParametricityLemmas where

open import Parametricity
open import HoTT hiding ( O; Path; _*_) renaming (! to rev)
-- (https://github.com/HoTT/HoTT-Agda)

-- Defining the operations in Moulin's thesis in terms of what we have
-- postulated:

_! : âˆ€ {â„“} {A : ğ•€ â†’ Set â„“} (u : (i : ğ•€) â†’ A i) â†’ u O âˆˆ i Â· (A i)
_! = lam

â¦…_,_â¦† : âˆ€ {â„“} {A : ğ•€ â†’ Set â„“} (a : A O) (p : a âˆˆ i Â· A i) â†’ ((i : ğ•€) â†’ A i)
â¦…_,_â¦† a p i = p * i

-- This inverse is the Î¨_A used in rule IN-PRED (cf. Moulin's thesis, p88)
Î¨ : âˆ€ {â„“} {A : Set â„“} (P : A â†’ Set â„“) â†’ A âˆˆ i Â· Set â„“
Î¨ P = embu-equiv .is-equiv.g P

-- This inverse is the Î¦_t used in rule IN-FUN (cf. Moulin's thesis, p88)
Î¦ : âˆ€ {â„“} {A : ğ•€ â†’ Set â„“} {B : (i : ğ•€) (x : A i) â†’ Set â„“}
  â†’ (t : (x : A O) â†’ B O x)
  â†’ (u : (x : (i : ğ•€) â†’ A i) â†’ (t (x O)) âˆˆ i Â· B i (x i))
  â†’ t âˆˆ i Â· ((x : A i) â†’ B i x)
Î¦ t u = embf-equiv t .is-equiv.g u

_â‹ˆ_ : âˆ€ {â„“} (A : Set â„“) (P : A â†’ Set â„“) (i : ğ•€) â†’ Set â„“
A â‹ˆ P = â¦… A , Î¨ P â¦†

â¦‰_,_â¦Š : âˆ€ {â„“} {A : ğ•€ â†’ Set â„“} {B : (i : ğ•€) (x : A i) â†’ Set â„“}
    â†’ (t : (x : A O) â†’ B O x)
    â†’ (u : (x : (i : ğ•€) â†’ A i) â†’ (t (x O)) âˆˆ i Â· B i (x i))
    â†’ (i : ğ•€) (x : A i) â†’ B i x
â¦‰ t , u â¦Š = â¦… t , Î¦ t u â¦†

-- Some lemmas for what follows
module _ where
  embu-inv : âˆ€ {â„“} {A : Set â„“}
    â†’ (A â†’ Set â„“) â†’ A âˆˆ i Â· Set â„“
  embu-inv {â„“} {A} = embu-equiv .is-equiv.g

  embu-fg : âˆ€ {â„“} {A : Set â„“} (P : A â†’ Set â„“)
    â†’ embu (embu-inv P) == P
  embu-fg {â„“} {A} = embu-equiv .is-equiv.f-g

  embu-coe : âˆ€ {â„“} {A : Set â„“} (P : A â†’ Set â„“) (a : A)
               â†’ P a â†’ embu (embu-inv P) a
  embu-coe P a p = coe (app= (rev (embu-fg P)) a) p

  embu-coe2 : âˆ€ {â„“} {A : Set â„“} (P : A â†’ Set â„“) (a : A)
              â†’ embu (embu-inv P) a â†’ P a
  embu-coe2 P a t = coe (app= (embu-fg P) a) t

  round-trip :  âˆ€ {â„“} {A : Set â„“} {P Q : A â†’ Set â„“}
    (Ï€ : P == Q) (a : A) (z : P a) â†’
    coe (app= (rev Ï€) a) (coe (app= Ï€ a) z) == z
  round-trip idp a z = idp

  round-trip2 :  âˆ€ {â„“} {A : Set â„“} {P Q : A â†’ Set â„“}
    (Ï€ : P == Q) (a : A) (z : Q a) â†’
    coe (app= Ï€ a) (coe (app= (rev Ï€) a) z) == z
  round-trip2 idp a z = idp

-- The conversion-relation axioms fall out of these definitions:
-- (cf. Moulin's thesis, p89)
PAIR-ORIG : {A : ğ•€ â†’ Set} (a : A O) (p : a âˆˆ i Â· A i) â†’
  â¦… a , p â¦† O == a
PAIR-ORIG a p = idp

PAIR-PARAM : {A : ğ•€ â†’ Set} (a : A O) (p : a âˆˆ i Â· A i) â†’
  (â¦… a , p â¦† !) == p
PAIR-PARAM a p = idp

SURJ-PARAM : {A : ğ•€ â†’ Set} (u : (i : ğ•€) â†’ A i) â†’
  â¦… u O , u ! â¦† == u
SURJ-PARAM u = idp

PAIR-PRED : âˆ€ {â„“} (A : Set â„“) (P : A â†’ Set â„“) (a : A) â†’
  P a == (a âˆˆ i Â· (A â‹ˆ P) i)
PAIR-PRED A P a = ua (equiv into out zig zag) where
  into : P a â†’ Path (A â‹ˆ P) a
  into = embu-coe P a
  out : Path (A â‹ˆ P) a â†’ P a
  out = embu-coe2 P a
  zig : (b : Path (A â‹ˆ P) a) â†’ into (out b) == b
  zig b = round-trip (embu-fg P) a b
  zag : (b : P a) â†’ out (into b) == b
  zag b = round-trip2 (embu-fg P) a b

PAIR-APP : âˆ€ {â„“} {A : ğ•€ â†’ Set â„“} {B : (i : ğ•€) (x : A i) â†’ Set â„“}
  â†’ (t : (x : A O) â†’ B O x)
  â†’ (u : (x : (i : ğ•€) â†’ A i) â†’ (t (x O)) âˆˆ i Â· B i (x i))
  â†’ (i : ğ•€) (a : (i : ğ•€) â†’ A i)
  â†’ â¦‰_,_â¦Š {B = B} t u i (a i) == â¦… t (a O) , u a â¦† i
PAIR-APP {B = B} t u i a = normalized-goal where
  before-ap : embf (is-equiv.g (embf-equiv t) u) a == u a
  before-ap = app= (embf-equiv {B = B} t .is-equiv.f-g u) a
  normalized-goal : (embf-equiv {B = B} t .is-equiv.g u * i) (a i) == (u a * i)
  normalized-goal = ap (Î» z â†’ z * i) before-ap

SURJ-TYPE : âˆ€ {â„“} (A : ğ•€ â†’ Set â„“) â†’
  Î¨ {A = A O} (Î» x â†’ x âˆˆ i Â· (A i)) == (A !)
SURJ-TYPE A = embu-equiv .is-equiv.g-f (lam A)

SURJ-FUN : âˆ€ {â„“} {A : ğ•€ â†’ Set â„“} {B : (i : ğ•€) (x : A i) â†’ Set â„“}
  â†’ (t : (i : ğ•€) (x : A i) â†’ B i x)
  â†’ Î¦ (t O) (Î» x â†’ (Î» i â†’ t i (x i)) !) == (t !)
SURJ-FUN {B = B} t = embf-equiv (t O) .is-equiv.g-f (lam t)
